formal-verification/lakefile.lean
@@ -9,7 +9,7 @@ require mathlib from git
   "https://github.com/leanprover-community/mathlib4.git"@"26d0eab43f05db777d1cf31abd31d3a57954b2a9"
 
 require ProvenZK from git
-  "https://github.com/reilabs/proven-zk.git"@"da07cc8facea04c379050624b5d8d1b45664b9af"
+  "https://github.com/reilabs/proven-zk.git"@"5f42162cb52c80315389c4f9a5d5e4782531e919"
 
 lean_lib FormalVerification {
   moreLeanArgs := #["--tstack=65520", "-DmaxRecDepth=10000", "-DmaxHeartbeats=200000000"]
